metatheory/weakeningScript.sml
@@ -412,6 +412,8 @@ res_tac >|
             tenv_ok_def, arithmeticTheory.ADD, arithmeticTheory.ADD_COMM],
  metis_tac [num_tvs_def, type_e_freevars, bind_tenv_def, bind_tvar_def,
             tenv_ok_def, arithmeticTheory.ADD, arithmeticTheory.ADD_COMM],
+ metis_tac [num_tvs_def, type_e_freevars, bind_tenv_def, bind_tvar_def,
+            tenv_ok_def, arithmeticTheory.ADD, arithmeticTheory.ADD_COMM],
  metis_tac [type_funs_Tfn, num_tvs_bind_var_list],
  metis_tac [type_funs_Tfn, num_tvs_bind_var_list, num_tvs_def,
             arithmeticTheory.ADD, arithmeticTheory.ADD_COMM],
@@ -452,58 +454,6 @@ rw [Once type_v_cases] >|
      metis_tac [],
  rw [bind_def, emp_def, bind_tvar_def, bind_tenv_def]]);
 
- (*
-val type_ctxt_weakening = Q.store_thm ("type_ctxt_weakening",
-`∀tvs tenvM tenvC tenvS tenv c t1 t2. type_ctxt tvs tenvM tenvC tenvS tenv c t1 t2 ⇒
-  !tenvM' tenvC' tenvS' tenv' tvs'.
-    tenvM_ok tenvM' ∧ tenv_ok tenv ∧ (num_tvs tenv = 0) ∧ ((tvs = 0) ∨ (tvs = tvs')) ∧ 
-    weakM tenvM' tenvM ∧ weakC tenvC' tenvC ∧ weakS tenvS' tenvS ∧ weak_tenvE tenv' tenv ⇒
-    type_ctxt tvs' tenvM' tenvC' tenvS' tenv' c t1 t2`,
-rw [type_ctxt_cases] >|
-[metis_tac [type_e_weakening, weak_tenvE_bind],
- metis_tac [type_e_weakening, weak_tenvE_bind],
- metis_tac [check_freevars_add, gt_0],
- metis_tac [check_freevars_add, gt_0, type_e_weakening, weak_tenvE_bind],
- metis_tac [type_e_weakening, weak_tenvE_refl],
- metis_tac [check_freevars_add, gt_0, type_v_weakening, weak_tenvE_bind],
- metis_tac [type_v_weakening],
- metis_tac [type_e_weakening],
- metis_tac [type_e_weakening],
- metis_tac [type_e_weakening],
- metis_tac [type_e_weakening],
- fs [RES_FORALL] >>
-     rw [] >-
-     metis_tac [check_freevars_add, gt_0] >>
-     PairCases_on `x` >>
-     rw [] >>
-     res_tac >>
-     fs [] >>
-     metis_tac [type_e_weakening, weak_tenvE_bind_var_list, type_p_weakening, gt_0],
- fs [RES_FORALL] >>
-     rw [] >>
-     PairCases_on `x` >>
-     rw [] >>
-     res_tac >>
-     fs [] >>
-     metis_tac [type_e_weakening, weak_tenvE_bind_var_list, type_p_weakening, DECIDE ``!x:num. x ≥ x``],
- metis_tac [check_freevars_add, gt_0, type_e_weakening, weak_tenvE_bind],
- metis_tac [type_e_weakening, weak_tenvE_bind],
- qexists_tac `ts1` >>
-     qexists_tac `ts2` >>
-     qexists_tac `t` >>
-     qexists_tac `tvs'` >>
-     rw [] >>
-     metis_tac [gt_0, check_freevars_add, EVERY_MEM, type_e_weakening,
-                weak_tenvE_bind_tvar2, type_v_weakening, weak_tenvC_lookup],
- qexists_tac `ts1` >>
-     qexists_tac `ts2` >>
-     qexists_tac `t` >>
-     qexists_tac `tvs'` >>
-     rw [] >>
-     metis_tac [gt_0, check_freevars_add, EVERY_MEM, type_e_weakening,
-                weak_tenvE_bind_tvar, type_v_weakening, weak_tenvC_lookup]]);
-                *)
-
 val type_ctxt_weakening = Q.store_thm ("type_ctxt_weakening",
 `∀tvs tenvM tenvC tenvS tenv c t1 t2. type_ctxt tvs tenvM tenvC tenvS tenv c t1 t2 ⇒
   !tenvM' tenvC' tenvS' tenv'.
@@ -528,6 +478,11 @@ rw [type_ctxt_cases] >|
      qexists_tac `ts2` >>
      qexists_tac `t` >>
      qexists_tac `tvs'` >>
+     rw [] >>
+     metis_tac [gt_0, check_freevars_add, EVERY_MEM, type_e_weakening,
+                weak_tenvE_bind_tvar, type_v_weakening, weak_tenvC_lookup],
+ qexists_tac `ts1` >>
+     qexists_tac `ts2` >>
      rw [] >>
      metis_tac [gt_0, check_freevars_add, EVERY_MEM, type_e_weakening,
                 weak_tenvE_bind_tvar, type_v_weakening, weak_tenvC_lookup]]);
